additions to bigint library

examples/stateful_bignum/carry_st.fst
@@ -12,16 +12,32 @@ open Axiomatic
 open Eval
 open Array
 
+
+val aux :
+  t:template -> bw_p_max:nat -> n:nat -> bwn:nat -> 
+  Tot nat
+let rec aux t bw_p_max n bwn =
+  if bwn >= bw_p_max then n
+  else aux t bw_p_max (n+1) (bwn + t n)
+
+
+(* Compute the required array length to store the carried result *)
+val compute_size :
+  a:bigint -> ST nat
+		 (requires (fun h -> True))
+		 (ensures (fun h0 n h1 -> True))
 let compute_size a =
   let bw = bitweight (Bigint63.t a) (get_length a) in
   let max = wordSize a in
   let bw_p_max = bw + max in
-  let rec aux t bw_p_max n bwn =
-    if bwn >= bw_p_max then n
-    else aux t bw_p_max (n+1) (bwn + t n) in
-  aux (Bigint63.t a) bw_p_max (get_length a) bwn
+  aux (Bigint63.t a) bw_p_max (get_length a) bw
 
-let carry_aux a i =
+val carry_aux :
+  a:bigint -> i:nat -> 
+  ST unit
+     (requires (fun h -> True))
+     (ensures (fun h0 u h1 -> True))
+let rec carry_aux a i =
   match get_length a - i - 1 with
   | 0 -> ()
   | _ -> 
@@ -38,6 +54,7 @@ let carry_aux a i =
      updateBigint a (i+1) th;
      carry_aux a (i+1)		  
 
+(* Perform a carry operations : the array is normalized but cells can have different sizes *)
 val carry : 
   a:bigint -> 
   ST unit
@@ -54,13 +71,13 @@ val carry :
      ))
 let carry a = 
   let size = compute_size a in
-  let new_array = Bigint.mk_zero_bigint size in
+  let new_array = Array.create size zero_tint in
   Array.blit (Bigint63.data a) 0 new_array 0 (get_length a);
-  Bigint63.data a := new_array;
+  Bigint63.data a := !new_array;
   carry_aux a 0
 
-	       
-val carry_mod:
+(* Carry modulo value *)	    
+assume val carry_mod:
   a:bigint -> m:bigint -> 
   ST bigint
      (requires (fun h -> 
@@ -82,7 +99,12 @@ val carry_mod:
 	       /\ (eval h1 b (getLength h1 b) = eval h0 a (getLength h0 a) % eval h0 m (getLength h0 m))
      ))
 
-let one_pass_carry_aux a len =
+val one_pass_carry_aux :
+  a:bigint -> len:nat -> 
+  ST unit
+     (requires (fun h -> True))
+     (ensures (fun h0 u h1 -> True))
+let rec one_pass_carry_aux a len =
   match len with
   | 0 -> ()
   | _ ->
@@ -95,10 +117,12 @@ let one_pass_carry_aux a len =
        erase (getSize h0 a i) in
      let size_aip =
        erase (getSize h0 a (i+1)) in
-     let high = shift_right ai (t i) in
+     let high = arithmetic_shift_right ai (t i) in
      (* Not constant time *)
      let low = signed_modulo ai (pow2 (t i)) in
-     let th = mk_tint a (max size_aip (wordSize a - t i) + 1) (Limb.add high (get a (i+1))) in
+     let aip1 = get a (i+1) in
+     let aip1 = Limb.add (t i) high (t (i+1)) aip1 in
+     let th = mk_tint a (max size_aip (wordSize a - t i) + 1) aip1 in
      let tl = mk_tint a (min size_ai (t i)) low in
      updateBigint a (i+1) th;
      updateBigint a i tl;
@@ -124,14 +148,151 @@ val one_pass_carry:
      ))
 let one_pass_carry a =
   let len = get_length a in
-  let array = Bigint.mk_zero_bigint (len + 1) in
+  let array = Array.create (len + 1) zero_tint in
   Array.blit (Bigint63.data a) 0 array 0 len;
   let last = get a (len-1) in
-  let t_last = Bigint63.t a (len-1)  
-  let high = shift_right last t_last in
+  let t_last = Bigint63.t a (len-1) in
+  let high = arithmetic_shift_right last t_last in
   let low = signed_modulo last (pow2 t_last) in
   let th = mk_tint a (wordSize a - t_last) high in
   let tl = mk_tint a t_last low in
   updateBigint a len th;
   updateBigint a (len-1) tl;
   one_pass_carry_aux a (len-1)
+
+(* Fully normal form for a big int : all cells have the same sign *)
+type FullyNormalized (h:heap) (b:bigint) =
+  (inHeap h b) 
+  /\ (forall (i:nat). i < getLength h b ==> getSize h b i <= Bigint63.t b i)
+  /\ ((exists (i:nat). (i < getLength h b /\ getValue h b i < 0))
+      ==> (forall (j:nat). j < getLength h b ==> getValue h b j <= 0))
+  /\ ((exists (i:nat). (i < getLength h b /\ getValue h b i > 0))
+      ==> (forall (j:nat). j < getLength h b ==> getValue h b j >= 0))
+
+(* Returns the sign of a bigint *)
+(* Not constant time *)
+val get_sign: a:bigint -> len:nat ->
+	      ST int
+		 (requires (fun h ->
+			    (Normalized h a)
+			    /\ (len <= getLength h a)
+		 ))
+		 (ensures (fun h0 s h1 ->
+			   (Normalized h0 a)
+			   /\ (len <= getLength h0 a)
+			   /\ (modifies !{} h0 h1)
+			   /\ (s = 0 \/ s = 1 \/ s = -1)
+			   /\ (s = 0 <==> eval h1 a (getLength h1 a) = 0)
+			   /\ (s = 1 <==> eval h1 a (getLength h1 a) > 0)
+			   /\ (s = -1 <==> eval h1 a (getLength h1 a) < 0)
+		 ))
+let rec get_sign a len =
+  match len with
+  | 0 -> 0
+  | _ -> 
+     let i = len - 1 in
+     let ai = get a i in
+     let s = IntLib.compare ai zero in
+     if s = 0 then get_sign a i else s
+
+(* Returns a fully normalized big int (all cells of the same sign) *)
+(* Not constant time *)
+val normalized_carry_aux :
+  a:bigint -> len:nat -> s:nat ->
+  ST unit
+     (requires (fun h -> 
+		(Normalized h a)
+		/\ (s = 0 \/ s = 1 \/ s = -1)
+		/\ (s = 0 <==> eval h a (getLength h a) = 0)
+		/\ (s = 1 <==> eval h a (getLength h a) > 0)
+		/\ (s = -1 <==> eval h a (getLength h a) < 0)
+		/\ (len <= getLength h a)
+		/\ (forall (i:nat).
+		    ((i < getLength h a /\ i >= len /\ s = 1) ==> getValue h a i >= 0)
+		    /\ ((i < getLength h a /\ i >= len /\ s = -1) ==> getValue h a i <= 0))
+     ))
+     (ensures (fun h0 u h1 ->
+	       (Normalized h0 a)
+	       /\ (modifies !{Bigint63.data a} h0 h1)
+	       /\ (getLength h1 a = getLength h0 a)
+	       /\ (eval h1 a (getLength h1 a) = eval h0 a (getLength h0 a))
+	       /\ (s = 0 \/ s = 1 \/ s = -1)
+	       /\ (s = 0 <==> eval h0 a (getLength h0 a) = 0)
+	       /\ (s = 1 <==> eval h0 a (getLength h0 a) > 0)
+	       /\ (s = -1 <==> eval h0 a (getLength h0 a) < 0)
+	       /\ (len <= getLength h0 a)
+	       /\ (FullyNormalized h1 a)
+     ))
+let rec normalized_carry_aux a len sign =
+  let minus_one = -1 in
+  match len with
+  | 0 -> ()
+  | _ ->
+     let i = len - 1 in
+     let ai = get a i in
+     match IntLib.compare ai zero with
+     | 0 -> 
+	(* The limb is zero, so we have to check that the cell bellow has the right sign *)
+	(* Otherwise, we swap is and change this limb value *)
+	if i = 0 then () (* least significant limb, nothing to do *)
+	else (
+	  let aim1 = get a (i-1) in
+	  let sm1 = IntLib.compare aim1 zero in
+	  if sign * sm1 >= 0 then () (* The adjacent lower cell has the right sign, all good *)
+	  else (
+	    (* Bad sign, change it *)
+	    if sign = 1 then (
+	      let ai = pow2 (Bigint63.t a i) - 1 in
+	      let ai = Bigint.mk_tint a (Bigint63.t a i) ai in
+	      let aim1 = aim1 + pow2 (Bigint63.t a (i-1)) in
+	      let aim1 = Bigint.mk_tint a (Bigint63.t a (i-1)) aim1 in
+	      Bigint.updateBigint a i ai;
+	      Bigint.updateBigint a (i-1) aim1)
+	    else (
+	      let ai = - (pow2 (Bigint63.t a i)) + 1 in
+	      let ai = Bigint.mk_tint a (Bigint63.t a i) ai in
+	      let aim1 = aim1 - pow2 (Bigint63.t a (i-1)) in
+	      let aim1 = Bigint.mk_tint a (Bigint63.t a (i-1)) aim1 in
+	      Bigint.updateBigint a i ai;
+	      Bigint.updateBigint a (i-1) aim1))
+	);
+	(* Iterate *)
+	normalized_carry_aux a i sign
+	
+     | 1 -> 
+	if sign = 1 then ()
+	else (
+	  let aip1 = get a len in
+	  let aip1 = Bigint.mk_tint a (Bigint63.t a len) (aip1 + 1) in
+	  let ai = Bigint.mk_tint a (Bigint63.t a i) (ai - pow2 (Bigint63.t a i)) in
+	  Bigint.updateBigint a len aip1;
+	  Bigint.updateBigint a i ai);
+	normalized_carry_aux a i sign
+
+     | minus_one -> 
+	if sign = 1 then ()
+	else (
+	  let aip1 = get a len in
+	  let aip1 = Bigint.mk_tint a (Bigint63.t a len) (aip1 - 1) in
+	  let ai = Bigint.mk_tint a (Bigint63.t a i) (ai + pow2 (Bigint63.t a i)) in
+	  Bigint.updateBigint a len aip1; 
+	  Bigint.updateBigint a i ai);
+	normalized_carry_aux a i sign
+
+
+
+(* Returns a fully normalized big int (all cells of the same sign) *)
+(* Not constant time *)
+val normalized_carry:
+  a:bigint -> 
+  ST unit
+     (requires (fun h -> (Normalized h a)
+     ))
+     (ensures (fun h0 u h1 ->
+	       (Normalized h0 a)
+	       /\ (modifies !{Bigint63.data a} h0 h1)
+	       /\ (FullyNormalized h1 a)
+     ))
+let normalized_carry a =
+  let sign = get_sign a (get_length a) in
+  normalized_carry_aux a (get_length a) sign
