examples/stateful_bignum/modulo_st.fst
@@ -4,7 +4,19 @@ open Heap
 open ST
 open Bigint
 open Eval
+open Shift
 
+(* The modulo pass goes as follows :
+   1 - shift the modulus by several cells so that its length is 1 less than a
+   2 - shift it by bits until it is bigger than the big int
+   3 - then subtract the modulus shifted by 1 bit less and iterate step 2
+   4 - when a < cell shifted modulus, iterate step 1 with a smaller shift
+Probably required for size : 
+  - Before each of steps 1, a carry
+  - Align the sign of the modulus on the sign of a
+ *)
+
+(* Expected specification for the modulo operation *)
 assume val modulo:
   a:bigint -> b:bigint -> 
   ST bigint
@@ -20,3 +32,79 @@ assume val modulo:
 	       /\ (getLength h1 a = getLength h0 b)
 	       /\ (eval h1 a (getLength h1 a) = eval h0 a (getLength h0 a) % eval h0 b (getLength h0 b))
      ))
+
+let rec modulo_bit a modulus shift =
+  (* Shift the modulus by "shift" bits *)
+  let s = shift_bits_over modulus shift in
+  (* If smaller than a iterate *)
+  if compare2 a s > 0 then 
+    modulo_bit a modulus (shift+1)
+  else (
+    (* Else if shift > 0 subtract modulus shifted by shift - 1 *)    
+    if shift > 0 then (
+      Substraction.substraction_with_lemma a (shift_bits_over modulus (shift-1));
+      modulo_bit a modulus 0
+    )
+    else 
+      (* Else return, a smaller than the modulus shifted by this number of cells *)
+      ()
+  ) 
+
+let modulo_cell a modulus offset =
+  match offset with
+  | 0 ->
+     (* Align modulus on the sign of a *)
+     let sign = 
+     let modulus = 
+       if get a (get_length a - 1) >= 0 /\ get modulus (get_length modulus - 1) >= 0 then
+	 modulus
+       else neg modulus in
+     (* Shift it bits by bits and subtract when required *)
+     modulo_bit a modulus 0;
+     (* a smaller than modulus, do final carry *)
+     carry a;
+     normalized_carry a
+  | _ ->
+     (* Align modulus on the sign of a *)
+     let modulus = 
+       if get a (get_length a - 1) >= 0 /\ get modulus (get_length modulus - 1) >= 0 then
+	 modulus
+       else neg modulus in
+     (* Shift by offset cells *)
+     let m = shift modulus offset in
+     (* Shift and subtract bit by bit *)
+     modulo_bit a m 0;
+     (* Carry *)
+     carry a;
+     normalized_carry a;
+     (* Iterate *)
+     modulo_cell a modulus offset
+
+(* A signed version of the modulo *)
+let signed_modulo a modulus =
+  (* Assume that the top cell of the modulus is not empty *)
+  (* Assume that the modulus is positive *)
+  let a = normalized_carry a in
+  let modulus = normalized_carry modulus in
+  let lmod = get_length modulus in
+  let la = get_length a in
+  if la < lmod then 
+    (* Since we assume top cell of modulus not empty, |a| < |modulus| so return a *)
+    Bigint.copy a
+  else 
+    let sign = compare2 a zero_bigint in
+    let a = if sign = -1 then neg a else a in
+    let b = Bigint.mk_zero_bigint (la + 1) in
+    Array.blit (Bigint63.data a) 0 (Bigint63.data b) 0 la;
+    modulo_cell b modulus (la - lmod);
+    let c = Array.make lmod zero_tint in
+    Array.blit (Bigint63.data b) 0 c 0 lmod;
+    Bigint63.data b := c;
+    if sign = -1 then neg b else b
+
+(* An unsigned version of the modulo *)
+let unsigned_modulo a modulus =
+  let b = signed_modulo a modulus in
+  if compare b zero_bigint = -1 then 
+    addition_with_lemma b modulus
+  else b
