examples/stateful_bignum/retemplate_st.fst
@@ -1,5 +1,6 @@
 module Retemplate 
 
+open IntLib
 open Heap
 open ST
 open Eval
@@ -32,15 +33,11 @@ val compute_size_aux : a:bigint -> t:template -> n:nat -> tn:nat -> wa:nat ->
 		       ST nat
 			  (requires (fun h -> True))
 			  (ensures (fun h0 n h1 -> True))
-let compute_size_aux a t n tn wa =
+let rec compute_size_aux a t n tn wa =
   if tn >= wa then n+1
   else compute_size_aux a t (n+1) (tn + t (n+1)) wa
 
 (* TODO : not verified *)
-val compute_size : a:bigint -> t:template ->
-		   ST nat
-		      (requires (fun h -> True))
-		      (ensures (fun h0 n h1 -> True))
 val compute_size : 
   a:bigint -> t:template ->
   ST nat
@@ -59,14 +56,14 @@ let compute_size a t =
   let n = 0 in
   let tn = t 0 in
   let weight_a = bitweight (Bigint63.t a) (get_length a) in
-  compute_size_aux a t tn tnp wa
+  compute_size_aux a t n tn weight_a
 
 (* TODO : not verified *)
 val retemplate_aux : a:bigint -> ta:template -> b:bigint -> tb:template -> len:nat ->
 		     ST unit
 			(requires (fun h -> True))
 			(ensures (fun h0 u h1 -> True))
-let retemplate_aux a ta b tb len =
+let rec retemplate_aux a ta b tb len =
   match get_length a - len with
   | 0 -> ()
   | _ ->
@@ -74,7 +71,7 @@ let retemplate_aux a ta b tb len =
      let tsize = ta len in
      let bw = bitweight ta len in
      fill_array b tb v tsize bw 0;
-     retemplate_aux a (len+1)
+     retemplate_aux a ta b tb (len+1)
 
 (* TODO : not verified *)
 val retemplate:
@@ -94,7 +91,8 @@ val retemplate:
 	       /\ (eval h1 b (getLength h1 b) = eval h0 a (getLength h0 a))
      ))
 let retemplate a t =
-  let new_size = comupte_size a t in
-  let b = Bigint63 (Bigint.mk_zero_bigint new_size) t in
-  retemplate_aux a (Bigint63.t a) b t 0
+  let new_size = compute_size a t in
+  let b = Bigint.mk_zero_bigint new_size t in
+  retemplate_aux a (Bigint63.t a) b t 0;
+  b
 
